Define Presburger sets as an abstract domain.

AbstractDomain.v
@@ -1,6 +1,6 @@
-Require Export PolyAI.TotalMap.
-Require Export Coq.Sets.Ensembles.
 Require Import PolyAI.SSA.
+Require Export PolyAI.Presburger.
+Require Export Coq.Sets.Ensembles.
 Require Import Coq.Program.Equality.
 Require Import Coq.Lists.List.
 From Coq Require Import ssreflect ssrfun ssrbool.
@@ -12,17 +12,59 @@ Open Scope string_scope.
 Class adom (ab:Type) :=
   {
     le : ab -> ab -> bool;
+    bot : ab;
     top : ab;
     join : ab -> ab -> ab;
 
+    gamma : ab -> Ensemble RegisterMap;
+
     le_refl: forall a, le a a = true;
     le_trans: forall a1 a2 a3, le a1 a2 = true -> le a2 a3 = true -> le a1 a3 = true;
-    gamma : ab -> Ensemble RegisterMap;
     gamma_monotone : forall a1 a2, le a1 a2 = true -> Included RegisterMap (gamma a1) (gamma a2);
     gamma_top : forall x, Ensembles.In RegisterMap (gamma top) x;
     join_sound_l : forall a1 a2, le a1 (join a1 a2);
     join_sound_r : forall a1 a2, le a2 (join a1 a2);
   }.
+
+
+(* Instance for the polyhedral abstract domain *)
+
+Theorem gamma_presburger_monotone {s: Type} (P : PresburgerSet s) :
+  forall p1 p2, is_subset p1 p2 = true ->
+           Included (string -> nat)
+                    (fun x => eval_point p1 x = true)
+                    (fun x => eval_point p2 x = true).
+Proof.
+  move => p1 p2 /is_subset_spec Hsubset x Hin.
+  rewrite /Ensembles.In in Hin *.
+  by apply Hsubset, Hin.
+Qed.
+
+Theorem gamma_presburger_top {s: Type} (P : PresburgerSet s) :
+  forall x, Ensembles.In (string -> nat) (eval_point universe_set) x.
+Proof.
+  move => x.
+  rewrite /Ensembles.In.
+  apply universe_set_spec.
+Qed.
+
+Instance PresburgerSetAD {s: Type} (P : PresburgerSet s) : adom s :=
+  {
+    le := is_subset;
+    bot := empty_set;
+    top := universe_set;
+    join := union_set;
+
+    gamma := eval_point;
+
+    le_refl := is_subset_refl P;
+    le_trans := is_subset_trans P;
+    gamma_monotone := gamma_presburger_monotone P;
+    gamma_top := gamma_presburger_top P;
+    join_sound_l := is_subset_union_l P;
+    join_sound_r := is_subset_union_r P;
+  }.
+
 
 (* Transfer functions for our language *)
 Class transfer_function {ab: Type} (A: adom ab) :=
