Presburger.v
@@ -1,4 +1,5 @@
 From Coq Require Import ssreflect ssrfun ssrbool.
+Require Export Coq.Sets.Ensembles.
 
 Require Import String.
 Open Scope string_scope.
@@ -7,6 +8,12 @@ Class PresburgerSet (s: Type) :=
   {
     eval_point : s -> (string -> nat) -> bool;
 
+    empty_set : s;
+    empty_set_spec : forall x, eval_point empty_set x = false;
+
+    universe_set : s;
+    universe_set_spec : forall x, eval_point universe_set x = true;
+
     union_set : s -> s -> s;
     union_set_spec : forall p1 p2 x,
         eval_point (union_set p1 p2) x = eval_point p1 x || eval_point p2 x;
@@ -14,4 +21,45 @@ Class PresburgerSet (s: Type) :=
     intersect_set : s -> s -> s;
     intersect_set_spec : forall p1 p2 x,
         eval_point (intersect_set p1 p2) x = eval_point p1 x && eval_point p2 x;
+
+    is_subset : s -> s -> bool;
+    is_subset_spec : forall p1 p2, is_subset p1 p2 = true <-> forall x, eval_point p1 x = true -> eval_point p2 x = true;
   }.
+
+
+Theorem is_subset_refl {s: Type} (P : PresburgerSet s) :
+  forall p, is_subset p p = true.
+Proof.
+  move => p.
+  apply is_subset_spec => //.
+Qed.
+
+Theorem is_subset_trans {s: Type} (P : PresburgerSet s) :
+  forall p1 p2 p3, is_subset p1 p2 = true ->
+              is_subset p2 p3 = true ->
+              is_subset p1 p3 = true.
+Proof.
+  move => p1 p2 p3 /is_subset_spec H12 /is_subset_spec H23.
+  apply is_subset_spec.
+  by auto.
+Qed.
+
+Theorem is_subset_union_l {s: Type} (P: PresburgerSet s ) :
+  forall p1 p2, is_subset p1 (union_set p1 p2).
+Proof.
+  move => p1 p2.
+  apply is_subset_spec => x Hp1.
+  rewrite union_set_spec Hp1.
+  reflexivity.
+Qed.
+
+Theorem is_subset_union_r {s: Type} (P: PresburgerSet s ) :
+  forall p1 p2, is_subset p2 (union_set p1 p2).
+Proof.
+  move => p1 p2.
+  apply is_subset_spec => x Hp2.
+  rewrite union_set_spec Hp2.
+  by apply orbT.
+Qed.
+
+
